Algebra.v
@@ -1,0 +1,648 @@
+From mathcomp Require Import all_ssreflect.
+Require Import PreOrders.
+Require Import Types.
+Require Import Cover.
+Require Import FCL.
+Require Import DependentFixpoint.
+
+Set Bullet Behavior "Strict Subproofs".
+
+Delimit Scope it_scope with IT.
+Open Scope it_scope.
+
+Delimit Scope alg_scope with ALG.
+Open Scope alg_scope.
+
+Import EqNotations.
+
+Notation "[ 'sort' c <= d ]" := (lessOrEqual c d) (at level 0, c at next level): alg_scope.
+
+Module SignatureFamily.
+  Record mixin_of (I: Type) (S: preOrdered) (O: finType): Type :=
+    Mixin {
+        arity: I -> O -> nat;
+        dom: forall i o, (arity i o).-tuple S;
+        range: I -> O -> S;
+      }.
+  Section ClassDef.
+    Structure class_of (I: Type) (S: Type) (O: Type) :=
+      Class {
+          sort_base: PreOrdered.class_of S;
+          operation_base: Finite.class_of O;  
+          mixin: mixin_of I
+                   (PreOrdered.Pack S sort_base)
+                   (@Finite.Pack O operation_base)
+        }.
+    Local Coercion operation_base : class_of >-> Finite.class_of.
+    Local Coercion sort_base : class_of >-> PreOrdered.class_of.
+    Structure type I := Pack { sort_sort : Type; operation_sort: Type; _ : class_of I sort_sort operation_sort }.
+    Variables (I: Type) (S: Type) (O: Type) (sigFam: type I).
+    Definition class := let: Pack _ _ c as sigFam' := sigFam return class_of I
+                                                                             (sort_sort I sigFam')
+                                                                             (operation_sort I sigFam')
+                        in c.
+    Definition clone c of phant_id class c := @Pack S O c.
+    Let xSort := (let: Pack S _ _ := sigFam in S).
+    Let xOperation := (let: Pack _ O _ := sigFam in O).
+    Notation xclass := (class : class_of I xSort xOperation).
+    Definition pack b0 b1 (m0: mixin_of I (PreOrdered.Pack S b1) (@Finite.Pack O b0)) :=
+      fun bSort bsort & phant_id (PreOrdered.class bSort) bsort =>
+        fun bOperation boperation & phant_id (Finite.class bOperation) boperation =>
+          fun m & phant_id m0 m => Pack I S O (@Class I S O bsort boperation m).
+
+    Definition operationEqType := Eval hnf in @Equality.Pack xOperation xclass.
+    Definition operationChoiceType := Eval hnf in  @Choice.Pack xOperation xclass.
+    Definition operationCountType := Eval hnf in  @Countable.Pack xOperation xclass.
+    Definition finType := Eval hnf in  @Finite.Pack xOperation xclass.
+
+    Definition sortEqType := Eval hnf in @Equality.Pack xSort (PreOrdered.base _ xclass).
+    Definition ctorCountType := Eval hnf in @Countable.Pack xSort (PreOrdered.base _ xclass).
+    Definition preOrdered := Eval hnf in  @PreOrdered.Pack xSort xclass.
+  End ClassDef.
+
+  Module Import Exports.
+    Coercion mixin: class_of >-> mixin_of.
+    Coercion preOrdered : type >-> PreOrdered.type.
+    Canonical preOrdered.
+    Coercion finType: type >-> Finite.type.
+    Canonical finType.
+
+    Notation sigFam := type.
+    Notation SignatureFamilyMixin := Mixin.
+    Notation SignatureFamilyType I S O m := (@pack I S O _ _ m _ _ id _ _ id m id).
+    Notation "[ 'sigFam' I 'of' S ',' O 'for' sigFam ]" :=
+      (@clone I S O sigFam _ idfun)
+        (at level 0, format "[ 'sigFam' I 'of' S ',' O 'for' sigFam ]") : form_scope.
+    Notation "[ 'sigFam' I 'of' S ',' O ]" :=
+      (@clone I S O _ _ id) (at level 0, format "[ 'sigFam' I 'of' S ',' O ]") : form_scope.
+  End Exports.
+End SignatureFamily.
+
+Export SignatureFamily.Exports.
+
+Definition sort {I: Type} (Sigma: sigFam I): preOrdered :=
+  SignatureFamily.preOrdered I Sigma.
+Definition operation {I: Type} (Sigma: sigFam I): finType :=
+  SignatureFamily.finType I (Sigma).
+Definition arity {I: Type} (Sigma: sigFam I): I -> operation Sigma -> nat :=
+  SignatureFamily.arity _ _ _ (SignatureFamily.class I Sigma).
+Definition dom {I: Type} (Sigma: sigFam I): forall (i: I) (o: operation Sigma), (arity Sigma i o).-tuple (sort Sigma) :=
+  SignatureFamily.dom _ _ _ (SignatureFamily.class I Sigma).
+Definition range {I: Type} (Sigma: sigFam I): I -> operation Sigma -> (sort Sigma) :=
+  SignatureFamily.range _ _ _ (SignatureFamily.class I Sigma).
+
+
+Definition sigFamSpec_Mixin {I: Type} {S: preOrdered} {O: finType} (spec: I -> O -> (seq S * S)):
+  SignatureFamily.mixin_of
+    I (PreOrdered.Pack S (PreOrdered.class S))
+    (Finite.Pack (Finite.class O)).
+Proof.
+  move: spec.
+  case: O => T1 o.
+  case: S => S c.
+  move => spec.
+  by exact: (@SignatureFamily.Mixin
+               I (PreOrdered.Pack S c) (Finite.Pack o)
+               (fun i o => seq.size (spec i o).1)
+               (fun i o =>
+                  let res := (spec i o).1 in
+                  @Tuple (seq.size res) S res (eq_refl _))
+               (fun i o => (spec i o).2)).
+Defined.
+
+Definition SigSpec I S O : Type := I -> O -> (seq S * S).
+Definition sigFamSpec_Type {I: Type} {S: preOrdered} {O: finType} (spec: SigSpec I S O) :=
+  Eval hnf in SignatureFamilyType I S O (sigFamSpec_Mixin spec).
+
+Record F {I: Type} (Sigma: sigFam I) (C: (sort Sigma) -> Type) (s: sort Sigma): Type :=
+    mkF {
+        index: I;
+        op: operation Sigma;
+        args: {ffun forall n, C (tnth (dom Sigma index op) n) };
+        range_cond: [sort (range Sigma index op) <= s]
+      }.
+
+Arguments mkF [I] [Sigma] [C] [s].
+Arguments index [I] [Sigma] [C] [s].
+Arguments op [I] [Sigma] [C] [s].
+Arguments args [I] [Sigma] [C] [s].
+Arguments range_cond [I] [Sigma] [C] [s].
+
+
+Section SignatureFunctor.
+  Variable I : Type.
+  Variable Sigma: sigFam I.
+  Variable C D: (sort Sigma) -> Type.
+  Definition fmap (f: forall s, C s -> D s): forall s, F Sigma C s -> F Sigma D s :=
+    fun s x => mkF (index x) (op x) [ffun n => f (tnth (dom Sigma (index x) (op x)) n) (args x n)] (range_cond x).
+End SignatureFunctor.
+
+Arguments fmap [I] [Sigma] [C D].
+
+Section SignatureFunctorProps.
+  Variable I : Type.
+  Variable Sigma: sigFam I.
+  Variable C D E: (sort Sigma) -> Type.
+
+  Lemma fmap_id: forall s, fmap (fun s => (@id (C s))) s =1 id.
+  Proof.
+    move => s.
+    rewrite /fmap.
+    case => /= *.
+    apply f_equal2 => //.
+    apply ffunP.
+    move => x.
+      by rewrite ffunE.
+  Qed.
+
+  Lemma fmap_comp: forall (f: forall s, D s -> E s) (g: forall s, C s -> D s) s, fmap (fun s => f s \o g s) s =1 fmap f s \o fmap g s.
+  Proof.
+    move => f g s.
+    rewrite /fmap /=.
+    case => /= *.
+    apply f_equal2 => //.
+    apply ffunP.
+    move => x.
+      by do 3 rewrite ffunE.
+  Qed.
+End SignatureFunctorProps.
+
+Module SigmaAlgebra.
+  Record mixin_of (I: Type) (Sigma: sigFam I) (C: (sort Sigma) -> Type): Type :=
+    Mixin { action: forall s, F Sigma C s -> C s }.
+  Section ClassDef.
+    Notation class_of := mixin_of.
+    Structure type I Sigma := Pack { carrier_sort : (sort Sigma) -> Type; _ : class_of I Sigma carrier_sort }.
+    Variables (I: Type) (Sigma: sigFam I) (C: (sort Sigma) -> Type) (alg: type I Sigma).
+    Definition class := let: Pack _ c as alg' := alg return class_of I Sigma (carrier_sort I Sigma alg') in c.
+    Definition clone c of phant_id class c := @Pack I Sigma C c.
+    Let xCarrier := (let: Pack C _ := alg in C).
+    Notation xclass := (class : class_of I xCarrier).
+    Definition pack (m0: mixin_of I Sigma C) :=
+          fun m & phant_id m0 m => Pack I Sigma C m.
+
+    Definition carrier := Eval hnf in xCarrier.
+  End ClassDef.
+
+  Module Import Exports.
+    Coercion carrier : type >-> Funclass.
+    Coercion action : mixin_of >-> Funclass.
+    
+    Notation sigAlg := (type _).
+    Notation Mixin := Mixin.
+    Notation AlgebraType I Sigma C m := (@pack I Sigma C m m id).
+    Notation "[ 'sigAlg' Sigma 'on' C 'for' sigAlg ]" :=
+      (@clone _ Sigma C sigAlg _ idfun)
+        (at level 0, format "[ 'sigAlg' Sigma 'on' C 'for' sigAlg ]") : form_scope.
+    Notation "[ 'sigAlg' Sigma 'on' C ]" :=
+      (@clone _ Sigma C _ _ id) (at level 0, format "[ 'sigAlg' Sigma 'on' C ]") : form_scope.
+  End Exports.
+End SigmaAlgebra.
+
+Export SigmaAlgebra.Exports.
+
+Definition carrier {I: Type} {Sigma: sigFam I} (alg: sigAlg Sigma): sort Sigma -> Type  :=
+  SigmaAlgebra.carrier I Sigma alg.
+Definition action {I: Type} {Sigma: sigFam I} (alg: sigAlg Sigma): forall s, F Sigma (carrier alg) s -> (carrier alg) s :=
+  SigmaAlgebra.action I (Sigma) (carrier alg) (SigmaAlgebra.class I Sigma alg).
+
+Coercion action: sigAlg >-> Funclass.
+
+Module SigmaCoAlgebra.
+  Record mixin_of (I: Type) (Sigma: sigFam I) (C: (sort Sigma) -> Type): Type :=
+    Mixin { coaction: forall s, C s -> F Sigma C s }.
+  Section ClassDef.
+    Notation class_of := mixin_of.
+    Structure type I Sigma := Pack { carrier_sort : (sort Sigma) -> Type; _ : class_of I Sigma carrier_sort }.
+    Variables (I: Type) (Sigma: sigFam I) (C: (sort Sigma) -> Type) (coAlg: type I Sigma).
+    Definition class := let: Pack _ c as coAlg' := coAlg return class_of I Sigma (carrier_sort I Sigma coAlg') in c.
+    Definition clone c of phant_id class c := @Pack I Sigma C c.
+    Let xCarrier := (let: Pack C _ := coAlg in C).
+    Notation xclass := (class : class_of I xCarrier).
+    Definition pack (m0: mixin_of I Sigma C) :=
+          fun m & phant_id m0 m => Pack I Sigma C m.
+
+    Definition carrier := Eval hnf in xCarrier.
+  End ClassDef.
+
+  Module Import Exports.
+    Coercion carrier : type >-> Funclass.
+    Coercion coaction : mixin_of >-> Funclass.
+    
+    Notation sigCoAlg := (type _).
+    Notation Mixin := Mixin.
+    Notation CoAlgebraType I Sigma C m := (@pack I Sigma C m m id).
+    Notation "[ 'sigCoAlg' Sigma 'on' C 'for' sigCoAlg ]" :=
+      (@clone I Sigma C sigCoAlg _ idfun)
+        (at level 0, format "[ 'sigCoAlg' Sigma 'on' C 'for' sigCoAlg ]") : form_scope.
+    Notation "[ 'sigCoAlg' Sigma 'on' C ]" :=
+      (@clone I Sigma C _ _ id) (at level 0, format "[ 'sigCoAlg' Sigma 'on' C ]") : form_scope.
+  End Exports.
+End SigmaCoAlgebra.
+
+Export SigmaCoAlgebra.Exports.
+
+Definition cocarrier {I: Type} {Sigma: sigFam I} (coAlg: sigCoAlg Sigma): sort Sigma -> Type  :=
+  SigmaCoAlgebra.carrier I Sigma coAlg.
+Definition coaction {I: Type} {Sigma: sigFam I} (coAlg: sigCoAlg Sigma):
+  forall s, cocarrier coAlg s -> F Sigma (cocarrier coAlg) s :=
+  SigmaCoAlgebra.coaction I (Sigma) (cocarrier coAlg) (SigmaCoAlgebra.class I Sigma coAlg).
+
+Coercion coaction: sigCoAlg >-> Funclass.
+
+Inductive AlgGen {I: Type} (Sigma: sigFam I) (h: sigAlg Sigma) (s: sort Sigma): carrier h s -> Prop :=
+| Gen : forall (x: F Sigma (carrier h) s),
+    (forall n, AlgGen Sigma h (tnth (dom Sigma (index x) (op x)) n) (args x n)) ->
+    AlgGen Sigma h s (action h s x).
+
+Section CanonicalAlgebraMorphism.
+  Variable I: Type.
+  Variable Sigma: sigFam I.
+  Variables h g: sigAlg Sigma.
+  Variable h_inv: forall s, carrier h s -> F Sigma (carrier h) s.
+
+  Variable A: Type.
+  Variable measure: forall (s: sort Sigma), carrier h s -> A.
+  Variable R: A -> A -> Prop.
+  Hypothesis R_wf: well_founded R.
+
+  Hypothesis h_inv_dec: forall s x n, R (measure _ (args (h_inv s x) n)) (measure s x).
+
+  Definition fmap_dec (m1: A) (f: forall s2 (y: carrier h s2), R (measure s2 y) m1 -> carrier g s2):
+    forall s (x: F Sigma (carrier h) s), (forall n, R (measure _ (args x n)) m1) -> F Sigma (carrier g) s :=
+    fun s x prfs => mkF (index x) (op x) [ffun n => f (tnth (dom Sigma (index x) (op x)) n)
+                                                  (args x n) (prfs n)] (range_cond x).
+
+  Definition canonical_morphism: forall s, carrier h s -> carrier g s :=
+    DepFix A R R_wf (sort Sigma) (carrier h) (fun s _ => carrier g s) measure
+           (fun s x canonical_morphism_rec =>
+              action g s (fmap_dec (measure s x) canonical_morphism_rec s (h_inv s x) (h_inv_dec s x))).
+          
+  
+  Lemma canonical_morphism_commutes:
+    forall s (x: carrier h s), canonical_morphism s x = action g s (fmap (canonical_morphism) s (h_inv s x)).
+  Proof.
+    move => s x.
+    rewrite /canonical_morphism /DepFix /=.
+    case: (R_wf (measure s x)) => prf /=.
+    apply: f_equal.
+    rewrite /fmap /fmap_dec -/canonical_morphism.
+    apply: (f_equal2 (mkF (index (h_inv s x)) (op (h_inv s x)))) => //.
+    apply: eq_dffun.
+    move => y /=.
+    apply: (fun f eqprf => Fix_F_inv A R (sort Sigma) (carrier h) (fun s _ => carrier g s) measure f eqprf
+                      (tnth (dom Sigma (index (h_inv s x)) (op (h_inv s x))) y)
+                      ((args (h_inv s x)) y)
+                      (prf (measure (tnth (dom Sigma (index (h_inv s x)) (op (h_inv s x))) y)
+                                      ((args (h_inv s x)) y)) (h_inv_dec s x y))
+                      (R_wf (measure (tnth (dom Sigma (index (h_inv s x)) (op (h_inv s x))) y)
+                                     ((args (h_inv s x)) y)))).
+    move => *.
+    apply: f_equal => //.
+    apply: f_equal2 => //.
+    apply ffunP.
+    move => z.
+      by do 2 rewrite ffunE.
+  Qed.
+
+  Variable hC: forall s, cancel (action h s) (h_inv s).
+  Variable h_invC: forall s, cancel (h_inv s) (action h s).
+
+  Lemma canonical_morphism_alg_morphism:
+    forall s, canonical_morphism s \o (action h s) =1 (action g s) \o fmap (canonical_morphism) s.
+  Proof.
+    move => s x.
+    rewrite /=.
+    rewrite canonical_morphism_commutes.
+      by rewrite hC.
+  Qed.
+
+  Lemma canonical_morphism_unique:
+    forall (m: forall s, carrier h s -> carrier g s) 
+      (is_alg_mor_m: forall s, m s \o (action h s) =1 (action g s) \o fmap m s),
+    forall s, canonical_morphism s =1 m s.
+  Proof.
+    move => m is_alg_mor_m s x.
+    rewrite canonical_morphism_commutes.
+    apply: (fun f_rec => Fix_F A R (sort Sigma) (carrier h)
+                            (fun s x => action g s (fmap canonical_morphism s (h_inv s x))  = m s x)
+                            measure f_rec s x (R_wf (measure s x))).
+    move: s x => _ _.
+    move => s x IH.
+    suff: (fmap canonical_morphism s (h_inv s x) = fmap m s (h_inv s x)).
+    { move => ->.
+      move: (is_alg_mor_m s (h_inv s x)).
+      rewrite /= => <-.
+        by rewrite h_invC. }
+    rewrite /fmap.
+    apply: f_equal2 => //.
+    apply ffunP.
+    move => n.
+    do 2 rewrite ffunE.
+    rewrite canonical_morphism_commutes.
+    apply: IH.
+      by apply: h_inv_dec.
+  Qed.
+
+  Lemma canonical_morphism_sound:
+    forall s x, AlgGen Sigma g s (canonical_morphism s x).
+  Proof.
+    move => s x.
+    rewrite canonical_morphism_commutes.
+    apply: (fun f_rec => Fix_F A R (sort Sigma) (carrier h)
+                            (fun s x => AlgGen Sigma g s (action g s (fmap canonical_morphism s (h_inv s x))))
+                            measure f_rec s x (R_wf (measure s x))).
+    move: s x => _ _.
+    move => s x.
+    move: (h_inv_dec s x).
+    case: (h_inv s x) => /= i o args range_prf dec_prf IH.
+    rewrite /fmap /=.
+    constructor.
+    move => /= n.
+    rewrite ffunE.
+    rewrite canonical_morphism_commutes.
+    apply: IH.
+      by apply: dec_prf.
+  Qed.
+
+   Lemma canonical_morphism_complete:
+    forall s x, AlgGen Sigma g s x -> exists y, canonical_morphism s y = x.
+  Proof.
+    move => s x prf.
+    elim: s x / prf.
+    move => s x prfs IH.
+    have: (exists f: {ffun forall n, carrier h (tnth (dom Sigma (index x) (op x)) n) },
+              forall n, canonical_morphism (tnth (dom Sigma (index x) (op x)) n) (f n) = (args x) n).
+    { move: IH.
+      clear ...
+      move: x => [] /= idx op args _ prf.
+      move: (fin_all_exists prf) => [] f f_prf.
+      exists (finfun f).
+      move => n.
+      rewrite ffunE.
+      apply: f_prf. }
+    move => [] args' args'_prf.
+    exists (action h s (mkF (index x) (op x) args' (range_cond x))).
+    move: (canonical_morphism_alg_morphism s (mkF (index x) (op x) args' (range_cond x))).
+    rewrite /= => ->.
+    apply f_equal.
+    rewrite /fmap /=.
+    move: args' args'_prf.
+    clear...
+    case: x => /= i o args range_cond args' args'_prf.
+    apply: f_equal2 => //.
+    apply ffunP.
+    move => n.
+    rewrite ffunE.
+      by apply: args'_prf.
+  Qed.
+End CanonicalAlgebraMorphism.
+
+Section FCLAlgebra.
+  Variable I: finType.
+  Variable Sigma: sigFam I.
+
+  Definition Combinator: finType := sum_finType I (operation Sigma).
+  Definition Constructor: ctor := sum_preOrderedType (diag_preOrderedType I) (sort Sigma).
+
+  Definition Gamma__I : {ffun I -> @IT Constructor} :=
+    [ffun i => Ctor (inl i) (Omega)].
+
+  Definition embed (s: sort Sigma): @IT Constructor := @Ctor Constructor (inr s) Omega.
+  Definition unembed (A: @IT Constructor): option (sort Sigma) :=
+    if A is Ctor (inr s) Omega then Some s else None.
+
+  Lemma embed_unembed: pcancel embed unembed.
+  Proof. done. Qed.
+
+  Lemma embed_le: forall s1 s2, [sort s1 <= s2] -> [bcd (embed s1) <= embed s2].
+  Proof.
+    move => s1 s2 prf.
+      by apply: BCD__CAx.
+  Qed.
+
+  Definition typeAtIndex (o: operation Sigma) (i: I) : @IT Constructor :=
+    (Gamma__I i) -> (mkArrow (rev (map embed (dom Sigma i o)), embed (range Sigma i o))).
+
+  Definition Gamma__Sigma : {ffun (operation Sigma) -> @IT Constructor} :=
+    [ffun o => \bigcap_(A_i <- map (typeAtIndex o) (enum I)) A_i].
+
+  Definition Gamma: {ffun Combinator -> @IT Constructor} :=
+    [ffun c => match c with
+              | inl idx => Gamma__I idx
+              | inr o => Gamma__Sigma o
+              end].
+
+  Definition C__FCL (s: sort Sigma) := { M : @Term Combinator | [FCL Gamma |- M : embed s] }.
+
+  Definition termAction__FCL (s: sort Sigma) (x: F Sigma C__FCL s): @Term Combinator :=
+    let: mkF i o args rangeprf := x in
+    revApply (Var (inr o) @ (Var (inl i)))
+             (rev (map (fun n => sval (args n)) (enum ('I_(arity Sigma i o))))).
+
+  Lemma proofAction__FCL: forall s x, [FCL Gamma |- termAction__FCL s x : embed s].
+  Proof.
+    move => s [] i o args range_prf.
+    have size_eq: (seq.size (rev (map (fun n => sval (args n)) (enum 'I_(arity Sigma i o)))) =
+                   seq.size (rev (map embed (dom Sigma i o)))).
+    { do 2 rewrite size_rev size_map.
+        by rewrite -cardE card_ord size_tuple. }
+    apply: (FCL__Sub (embed (range Sigma i o))); last by apply: embed_le.    
+    apply: (FCL__App Gamma (@Var Combinator (inr o) @ Var (inl i))
+                   (rev (map (fun n => sval (args n)) (enum ('I_(arity Sigma i o)))))
+                   (rev (map embed (dom Sigma i o)), embed (range Sigma i o))) => //.
+    rewrite /=.
+    move => n.
+    case arity0: (n < (arity Sigma i o)).
+    - rewrite nth_rev; last first.
+      { by rewrite size_map -cardE card_ord. }
+      rewrite nth_rev; last first.
+      { by rewrite size_map size_tuple. }
+      rewrite (nth_map s); last first.
+      { by rewrite size_map size_tuple -subn_gt0 subnBA // addnC -addnBA // subnn. }
+      rewrite (nth_map (Ordinal arity0)); last first.
+      { rewrite size_map size_tuple card_ord -subn_gt0 subnBA // addnC -addnBA // subnn. }
+      rewrite size_map.
+      move: (args
+               (nth (Ordinal arity0)
+                    (enum 'I_(arity Sigma i o))
+                    (seq.size (enum 'I_(arity Sigma i o)) - n.+1))).
+      move => [] M /=.
+      rewrite (tnth_nth s).
+      rewrite (@nth_enum_ord _ (Ordinal arity0) ((seq.size (enum 'I_(arity Sigma i o)) - n.+1))); last first.
+      { by rewrite -cardE card_ord -subn_gt0 subnBA // addnC -addnBA // subnn. }
+      move: size_eq.
+        by rewrite size_rev size_rev size_map => ->.
+    - rewrite nth_default; last first.
+      { by rewrite size_rev size_map -cardE card_ord leqNgt arity0. }
+      rewrite nth_default; last first.
+      { by rewrite size_rev size_map size_tuple leqNgt arity0. }
+      apply: FCL__MP; last by apply: FCL__Var.
+      apply: FCL__Sub; first by apply: FCL__Var.
+      rewrite /Gamma ffunE /Gamma__Sigma ffunE ffunE.
+      apply: BCD__Trans.
+      + apply: (bcd_subset_f _ id _ [:: typeAtIndex o i]).
+        move => x.
+        rewrite mem_seq1.
+        move => /eqP ->.
+        apply /mapP.
+        exists i => //.
+          by rewrite mem_enum.
+      + rewrite /= /typeAtIndex.
+          by apply: BCD__Sub.
+  Qed.
+
+  Definition action__FCL (s: sort Sigma) (x: F Sigma C__FCL s): C__FCL s :=
+    exist _ (termAction__FCL s x) (proofAction__FCL s x).
+
+  Definition termCoAction__FCL (s: sort Sigma) (x: C__FCL s): seq (@Term Combinator) :=
+    behead (unapply (sval x)).2.
+
+  Lemma mkArrow__Omega {C: ctor}: forall srcs (A: @IT C), isOmega (mkArrow (srcs, A)) = isOmega A.
+  Proof.
+    elim /last_ind => // srcs src IH.
+    move => A /=.
+    rewrite mkArrow_rcons /=.
+      by apply: IH.
+  Qed.
+
+  Lemma unapplyNotIndex: forall s (x: C__FCL s), if (unapply (sval x)).1 is (inl _) then False else True.
+  Proof.
+    move => s [] M.
+    rewrite -(unapply_revapply M) /= revapply_unapply.
+    move => /FCL__invApp [] srcs [] size__eq /(fun prf => prf (seq.size srcs)).
+    rewrite nth_default; last by rewrite size__eq.
+    rewrite nth_default //.
+    case: (unapply M).1 => //.
+    move => i /minimalType_minimal.
+    move: size__eq => _.
+    elim /last_ind: srcs.
+    - move => /subty_complete.
+      rewrite /mkArrow /= /embed /= ffunE /Gamma__I ffunE.
+      move => /SubtypeMachine_inv /= /(fun prf => prf (fun i r => if r is Return true then false else true)) res.
+        by move: (res (fun _ _ => isT)).
+    - move => srcs src _.
+      rewrite mkArrow_rcons.
+      move => /subty_complete.
+      rewrite /= /Gamma ffunE /Gamma__I ffunE.
+      move => /SubtypeMachine_inv /(fun prf => prf (fun i r => if r is Return true then false else true)) res.
+      suff: false by done.
+      apply: res.
+      move => Delta r'.
+      rewrite /cast /= mkArrow__Omega /=.
+      move => /emptyDoneTgt -> /=.
+      case: r' => //.
+      move => /Omega__subty.
+      rewrite mkArrow__Omega /=.
+      move => res.
+        by apply: res.
+  Qed.
+
+  Definition opCoAction__FCL (s: sort Sigma) (x: C__FCL s): operation Sigma :=
+    match (unapply (sval x)).1 as o return (if o is (inl _) then False else True) -> operation Sigma with
+    | inl _ => False_rect _
+    | inr o => fun _ => o
+    end (unapplyNotIndex s x).
+
+  Lemma 
+
+  Lemma indexType_sound: forall M i, [FCL Gamma |- M : @Ctor Constructor (inl i) Omega] -> M = (@Var Combinator (inl i)).
+  Proof.
+    move => M i.
+    move A__eq: (@Ctor Constructor (inl i) Omega) => A prf.
+    move: i A__eq.
+    elim /FCL_normalized_ind: M A /prf.
+    - case.
+      + move => i1 i2.
+        rewrite /Gamma ffunE /Gamma__I ffunE.
+          by move => [] ->.
+      + move => o i.
+        rewrite /Gamma ffunE /Gamma__Sigma ffunE.
+          by case: (enum I) => // ? [] //.
+    - move => c A IH prf i A__eq.
+      apply: IH.
+      move: prf.
+      rewrite -A__eq /Gamma ffunE.
+      case: c.
+      + move => i2.
+        rewrite /Gamma__I ffunE.
+        move => /subty_complete /SubtypeMachine_inv /=.
+        move => /(fun prf => prf (fun i r => if (i, r) is ([subty (Ctor (inl i1) Omega) of (Ctor (inl i2) Omega)], Return true)
+                                      then i2 = i1 else True)) => res.
+        apply: f_equal2 => //.
+        apply: f_equal.
+        apply: res.
+        rewrite /cast /=.
+        case res: (i2 == i).
+        * rewrite (eqP res) preorder_reflexive.
+            by case.
+        * by rewrite /[sort _ <= _] /= /[sort _ <= _] /= res.
+      + move => o /subty_complete /SubtypeMachine_inv /(fun prf => prf (fun i r => if r is Return true then false else true)) res.
+        suff: false by done.
+        apply: res.
+        rewrite /Gamma__Sigma ffunE.
+        suff: nilp (cast (@Ctor Constructor (inl i) Omega) (\bigcap_(A_i <- map (typeAtIndex o) (enum I)) A_i)) by move => ->.
+        rewrite slow_cast_cast.
+        elim: (enum I) => // idx idxs.
+          by case: idxs => [].
+    - 
+
+
+      
+
+
+
+  Lemma indexType_src: forall o N Ns A, ~~isOmega A -> [FCL Gamma |- revApply (Var (inr o)) Ns : A] -> 
+
+  Lemma unapplyIsIndex: forall s (x: C__FCL s), if (unapply (sval x)).2 is [:: (Var (inl _)) & _] then True else False.
+  Proof.
+    move => s x.
+    move: (unapplyNotIndex s x).
+    case x => M.
+    rewrite -(unapply_revapply M) /= revapply_unapply.
+    move => /FCL__invApp [] srcs [] size__eq.
+    case: (unapply M).1 => // o.
+    move: size__eq.
+    case: (unapply M).2.
+    - case: srcs => // _.
+      move => /(fun prf => prf 0) /=.
+      move => /minimalType_minimal /=.
+      rewrite /mkArrow /= /Gamma ffunE /Gamma__Sigma ffunE /embed.
+      move => /subty_complete /SubtypeMachine_inv /= /(fun prf => prf (fun i r => if r is Return true then false else true)) res.
+      suff: false by done.
+      apply: res.
+      suff: (nilp (cast (@Ctor Constructor (inr s) Omega) (\bigcap_(A_i <- map (typeAtIndex o) (enum I)) A_i))) by move ->.
+      rewrite slow_cast_cast.
+      elim (enum I) => // idx idxs.
+        by case: idxs.
+    - case: srcs => // src srcs.
+      move => N Ns _ prf.
+      have src__geq: [src 
+
+      
+      
+
+
+      
+
+  
+
+  Lemma proofCoAction__FCL (s: sort Sigma) (x: C__FCL s):
+    forall n, [FCL Gamma |- (nth (opCoAction__FCL s x) (termCoAction__FCL s x) n) :
+                       (nth (Gamma (opCoAction__FCL s x)) (dom Sigma )
+                                                                                                                                  
+
+    let: mkF i o args rangeprf := x in
+    revApply (Var (inr o) @ (Var (inl i)))
+             (rev (map (fun n => sval (args n)) (enum ('I_(arity Sigma i o))))).
+
+
+
+
+
+                           
+
+
+  
+
+
