DependentFixpoint.v
@@ -1,0 +1,43 @@
+(* Fix_F with heterogenious type dependent arguments *)
+
+Section DependentFixPoint.
+  Variable A: Type.
+  Variable R: A -> A -> Prop.
+  Variable Rwf: well_founded R.
+  
+  Variable T: Type.
+  Variable TT: T -> Type.
+  
+  Variable P : forall (t: T), TT t -> Type.
+  Variable f : forall (t: T), TT t -> A.
+  Variable F : forall (t : T),
+      forall (x : TT t),
+        (forall (t' : T) (y : TT t'),
+            R (f t' y) (f t x) -> P t' y) -> P t x.
+
+  Fixpoint Fix_F (t: T) (x: TT t) (a: Acc R (f t x)) : P t x :=
+    F t x (fun (t' : T) (y : TT t') (h : R (f t' y) (f t x)) =>
+             Fix_F t' y (Acc_inv a h)).
+
+  Definition DepFix (t: T) (x: TT t) := Fix_F t x (Rwf (f t x)).
+
+
+  Hypothesis
+    F_ext :
+      forall (t: T) (x: TT t) (g g': forall (t': T) (y: TT t'), R (f t' y) (f t x) -> P t' y),
+        (forall (t': T) (y: TT t') (p: R (f t' y) (f t x)), g t' y p = g' t' y p) -> F t x g = F t x g'.
+
+  Fixpoint Fix_F_inv (t: T) (x: TT t) (r s: Acc R (f t x)) { struct r}: Fix_F t x r = Fix_F t x s.
+  Proof.
+    destruct r.
+    destruct s.
+    simpl.
+    match goal with
+    |[|- F t x ?lhs = F t x ?rhs ] =>
+     apply (F_ext t x lhs rhs)
+    end.
+    intros.
+    apply Fix_F_inv.
+  Qed.
+  
+End DependentFixPoint.    
