PreOrdered.v
@@ -1,0 +1,107 @@
+From mathcomp Require Import all_ssreflect.
+
+Set Bullet Behavior "Strict Subproofs".
+
+Module PreOrdered.
+  Definition preorder (preOrdered: Type) := (preOrdered -> preOrdered -> bool)%type.
+  Definition preorder_reflexive (preOrdered: Type) (lessOrEqual: preorder preOrdered): Type :=
+    forall c, lessOrEqual c c = true.
+
+  Definition preorder_transitive (preOrdered: Type) (lessOrEqual: preorder preOrdered): Type :=
+    forall (c: preOrdered) (d: preOrdered) (e: preOrdered),
+      lessOrEqual c d && lessOrEqual d e ==> lessOrEqual c e.
+
+  Record mixin_of (preOrdered: Type): Type :=
+    Mixin {
+        lessOrEqual : preorder preOrdered;
+        _: preorder_reflexive preOrdered lessOrEqual;
+        _: preorder_transitive preOrdered lessOrEqual
+      }.
+
+  Section ClassDef.
+    Record class_of (C: Type) :=
+      Class {
+          base: Countable.class_of C;
+          mixin: mixin_of C
+        }.
+    Local Coercion base : class_of >-> Countable.class_of.
+    Structure type: Type := Pack { sort : Type; _ : class_of sort }.
+    Local Coercion sort : type >-> Sortclass.
+    Variables (T: Type) (cPreOrdered: type).
+    Definition class := let: Pack _ c as cPreOrdered' := cPreOrdered return class_of cPreOrdered' in c.
+    Definition clone c of phant_id class c := @Pack T c.
+    Let xT := let: Pack T _ := cPreOrdered in T.
+    Notation xclass := (class : class_of xT).
+    Definition pack m :=
+      fun b bT & phant_id (Countable.class bT) b => Pack _ (@Class T b m).
+    Definition eqType := Eval hnf in @Equality.Pack cPreOrdered xclass.
+    Definition choiceType := Eval hnf in  @Choice.Pack cPreOrdered xclass.
+    Definition countType := Eval hnf in @Countable.Pack cPreOrdered xclass.
+  End ClassDef.
+
+  Module Import Exports.
+    Coercion base : class_of >-> Countable.class_of.
+    Coercion mixin: class_of >-> mixin_of.
+    Coercion sort : type >-> Sortclass.
+    Coercion eqType : type >-> Equality.type.
+    Canonical eqType.
+    Coercion choiceType : type >-> Choice.type.
+    Canonical choiceType.
+    Coercion countType : type >-> Countable.type.
+    Canonical countType.
+
+    Notation preOrdered := type.
+    Notation PreOrderedType C m := (@pack C m _ _ id).
+    Notation PreOrderedMixin := Mixin.
+
+    Notation "[ 'preOrderedType' 'of' T 'for' cT ]" :=
+      (@clone T cT _ idfun) (at level 0, format "[ 'preOrderedType' 'of' T 'for' cT ]") : form_scope.
+    Notation "[ 'preOrderedType' 'of' T ]" :=
+      (@clone T _ _ id) (at level 0, format "[ 'preOrderedType' 'of' T ]") : form_scope.
+  End Exports.
+End PreOrdered.
+Export PreOrdered.Exports.
+
+Definition lessOrEqual c := PreOrdered.lessOrEqual _ (PreOrdered.class c).
+Arguments lessOrEqual [c].
+
+Lemma preorder_reflexive c: PreOrdered.preorder_reflexive _ (@lessOrEqual c).
+Proof. by case c => ? [] ? []. Qed.
+Arguments preorder_reflexive [c].
+Lemma preorder_transitive c: PreOrdered.preorder_transitive _ (@lessOrEqual c).
+Proof. by case c => ? [] ? []. Qed.
+Arguments preorder_transitive [c].
+
+Section NatPreOrdered.
+  Lemma leq_transb: forall (m n p: nat), (m <= n) && (n <= p) ==> (m <= p).
+  Proof.
+    move => m n p.
+    move: (@leq_trans n m p).
+    case (m <= n) => //=.
+    case (n <= p) => //= prf.
+      by apply: prf.
+  Qed.
+
+  Definition nat_preOrderedMixin := PreOrdered.Mixin nat leq leqnn leq_transb.
+  Canonical nat_preOrderedType := Eval hnf in PreOrderedType nat nat_preOrderedMixin.
+End NatPreOrdered.
+
+Section DiagCountTypePreOrdered.
+  Variable T: countType.  
+
+  Lemma eqop_refl: PreOrdered.preorder_reflexive _ (@eq_op T).
+  Proof.
+    move => x.
+      by rewrite eq_refl.
+  Qed.
+
+  Lemma eqop_trans: PreOrdered.preorder_transitive _ (@eq_op T).
+  Proof.
+    move => x y z.
+    apply /implyP.
+      by move => /andP [] /eqP ->.
+  Qed.
+
+  Definition diag_preOrderedMixin := PreOrdered.Mixin T eq_op eqop_refl eqop_trans.
+  Definition diag_preOrderedType := Eval hnf in PreOrderedType T diag_preOrderedMixin.
+End DiagCountTypePreOrdered.
