default.nix
@@ -2,16 +2,34 @@ let
   pkgs = import <nixpkgs>{}; 
 in 
 { stdenv ? pkgs.stdenv,
-  coq ? pkgs.coq_8_9,
+  coq ? pkgs.coq_8_8,
   gnumake ? pkgs.gnumake,
-  coqPackages ? pkgs.coqPackages_8_9 }:
+  coqPackages ? pkgs.coqPackages_8_8,
+  ncurses ? pkgs.ncurses,
+  which ? pkgs.which,
+  graphviz ? pkgs.graphviz,
+  fetchFromGitHub ? pkgs.fetchFromGitHub,
+}:
   #let
     #inherit (coqPackages) autosubst;
     #in
+
+let
+  mkChicken' = self: coq:
+    let callPackage = pkgs.newScope self ; in rec {
+      inherit callPackage coq;
+      coqPackages = self;
+      camlp5 = pkgs.ocamlPackages.camlp5_6_strict;
+      mathcomp = callPackage ./mathcomp.nix { };
+    };
+  mkChicken = coq: let self = mkChicken' self coq; in self;
+  lecoq = mkChicken coq;
+  mathcomp = lecoq.mathcomp;
+in
 stdenv.mkDerivation rec {
   name = "Thesis";
   version = "0.0.1";
   src = ./.;
-  buildInputs = [ coq coqPackages.mathcomp ];
+  buildInputs = [ coq mathcomp ];
   buildTools = [ gnumake ];
 }
